stlc/soundness.v
@@ -5,27 +5,17 @@ From iris.program_logic Require Import adequacy.
 Section soundness.
   Let Σ := #[].
 
-  Lemma empty_env_subst e : e.[env_subst []] = e.
-  Proof. change (env_subst []) with ids. by asimpl. Qed.
-
   Lemma wp_soundness e τ : [] ⊢ₜ e : τ → True ⊢ WP e {{ @interp (globalF Σ) τ }}.
   Proof.
-    iIntros {H} "".
-    rewrite -(empty_env_subst e).
-    iApply typed_interp; eauto.
+    iIntros {H} "". rewrite -(empty_env_subst e). iApply typed_interp; eauto.
   Qed.
 
-  Theorem Soundness e τ :
-    [] ⊢ₜ e : τ →
-    ∀ e' thp, rtc step ([e], tt) (e' :: thp, tt) →
-              ¬ reducible e' tt → is_Some (to_val e').
+  Theorem soundness e τ e' thp :
+    [] ⊢ₜ e : τ → rtc step ([e], ()) (e' :: thp, ()) →
+    is_Some (to_val e') ∨ reducible e' ().
   Proof.
-    intros H1 e' thp Hstp Hnr.
-    apply wp_soundness in H1.
-    edestruct(@wp_adequacy_reducible lang (globalF Σ) ⊤
-                                     (interp τ) e e' (e' :: thp) tt ∅)
-      as [Ha|Ha]; eauto using ucmra_unit_valid; try tauto.
-    - iIntros "H". iApply H1.
+    intros. eapply wp_adequacy_reducible; eauto using ucmra_unit_valid.
+    - iIntros "H". by iApply wp_soundness.
     - constructor.
   Qed.
 End soundness.
